@prefix : <https://ontologies.msaas.me/fmi-ontology.ttl#> .
@prefix owl: <http://www.w3.org/2002/07/owl#> .
@prefix rdf: <http://www.w3.org/1999/02/22-rdf-syntax-ns#> .
@prefix sms: <https://ontologies.msaas.me/sms-ontology.ttl#> .
@prefix xml: <http://www.w3.org/XML/1998/namespace> .
@prefix xsd: <http://www.w3.org/2001/XMLSchema#> .
@prefix rdfs: <http://www.w3.org/2000/01/rdf-schema#> .
@base <https://ontologies.msaas.me/fmi-ontology.ttl> .

<https://ontologies.msaas.me/fmi-ontology.ttl> rdf:type owl:Ontology .

#################################################################
#    Object Properties
#################################################################

###  https://ontologies.msaas.me/fmi-ontology.ttl#copyright
:copyright rdf:type owl:ObjectProperty ;
           rdfs:domain :FMU ;
           rdfs:comment "Optional string with the name and organization of the model author."@en .


###  https://ontologies.msaas.me/fmi-ontology.ttl#description
:description rdf:type owl:ObjectProperty ;
             rdfs:domain :FMU ;
             rdfs:comment "Optional string with a brief description of the model."@en .


###  https://ontologies.msaas.me/fmi-ontology.ttl#fmiVersion
:fmiVersion rdf:type owl:ObjectProperty ;
            rdfs:domain :FMU ;
            rdfs:comment """Version of “FMI for Model Exchange or Co-Simulation” that was used to generate the XML file."""@en .


###  https://ontologies.msaas.me/fmi-ontology.ttl#generationDateAndTime
:generationDateAndTime rdf:type owl:ObjectProperty ;
                       rdfs:domain :FMU ;
                       rdfs:comment "Optional date and time when the XML file was generated."@en ,
                                    "The format is a subset of “xs:dateTime” and should be: “YYYY-MM-DDThh:mm:ssZ\" (with one “T” between date and time; “Z” characterizes the Zulu time zone, in other words Greenwich meantime)."@en .


###  https://ontologies.msaas.me/fmi-ontology.ttl#generationTool
:generationTool rdf:type owl:ObjectProperty ;
                rdfs:domain :FMU ;
                rdfs:comment "Optional name of the tool that generated the XML file."@en .


###  https://ontologies.msaas.me/fmi-ontology.ttl#guid
:guid rdf:type owl:ObjectProperty ;
      rdfs:domain :FMU ;
      rdfs:comment """The “Globally Unique IDentifier” is a string that is used to check that the XML file is compatible with the C functions of the FMU."""@en .


###  https://ontologies.msaas.me/fmi-ontology.ttl#license
:license rdf:type owl:ObjectProperty ;
         rdfs:domain :FMU ;
         rdfs:comment "Optional information on the intellectual property licensing for this FMU."@en .


###  https://ontologies.msaas.me/fmi-ontology.ttl#modelName
:modelName rdf:type owl:ObjectProperty ;
           rdfs:domain :FMU ;
           rdfs:comment "The name of the model as used in the modeling environment that generated the XML file, such as \"Modelica.Mechanics.Rotational.Examples.CoupledClutches”."@en .


###  https://ontologies.msaas.me/fmi-ontology.ttl#numberOfEventIndicators
:numberOfEventIndicators rdf:type owl:ObjectProperty ;
                         rdfs:domain :FMU ;
                         rdfs:comment """The (fixed) number of event indicators for an FMU based on FMI for Model Exchange. For Co-Simulation, this value is ignored."""@en .


###  https://ontologies.msaas.me/fmi-ontology.ttl#version
:version rdf:type owl:ObjectProperty ;
         rdfs:domain :FMU .


#################################################################
#    Classes
#################################################################

###  https://ontologies.msaas.me/fmi-ontology.ttl#FMU
:FMU rdf:type owl:Class ;
     rdfs:comment "An executable implementation of the Functional Mock-up Interface (FMI): a Functional Mock-up Unit (FMU)."@en .


###  Generated by the OWL API (version 4.5.9.2019-02-01T07:24:44Z) https://github.com/owlcs/owlapi
